src/graph_theory/k4.lean
@@ -1,0 +1,182 @@
+import tactic
+import combinatorics.simple_graph.basic
+import graph_theory.planar
+
+namespace simple_graph
+
+def K4 := complete_graph (finset.range 4)
+
+def K4_to_plane (v : finset.range 4) : (ℤ × ℤ) :=
+begin
+  cases v with v' hv',
+  exact if v'=0 then (0,0) else
+        if v'=1 then (0,1) else
+        if v'=2 then (0,2) else (1,1),
+end
+
+lemma out_of_range (x : ℕ) : x.succ.succ.succ.succ ∉ finset.range 4 :=
+begin
+  intro h,
+  rw finset.mem_range at h,
+  change x.succ.succ.succ.succ with x + 4 at h, 
+  linarith,
+end
+
+def K4_dart_to_path (e : K4.dart) : plane.walk (K4_to_plane e.fst) (K4_to_plane e.snd) :=
+begin
+  cases e.fst with x hx,
+  cases e.snd with y hy,
+
+  iterate 4 { any_goals { cases x, norm_num, }, },
+  iterate 4 { any_goals { cases y, norm_num, }, },
+
+  any_goals {
+    exfalso, 
+    { apply out_of_range x, assumption, } <|> { apply out_of_range y, assumption, }
+  },
+
+  all_goals { 
+    rw [K4_to_plane, K4_to_plane],
+    simp only [nat.one_ne_zero,
+     zero_eq_bit0,
+     bit0_eq_zero,
+     nat.bit1_ne_bit0,
+     nat.bit1_eq_one,
+     if_true,
+     eq_self_iff_true,
+     nat.zero_ne_one,
+     if_false,
+     nat.succ_succ_ne_one,
+     nat.bit1_ne_zero],
+  },
+
+  any_goals { exact walk.cons (by rw [plane, cartesian_product, Z]; norm_num) walk.nil, },
+  
+  have step1 : plane.adj (0,0) (-1,0) := by rw [plane, cartesian_product, Z]; norm_num,
+  have step2 : plane.adj (-1,0) (-1,1) := by rw [plane, cartesian_product, Z]; norm_num,
+  have step3 : plane.adj (-1,1) (-1,2) := by rw [plane, cartesian_product, Z]; norm_num,
+  have step4 : plane.adj (-1,2) (0,2) := by rw [plane, cartesian_product, Z]; norm_num,
+  exact walk.cons step1 (walk.cons step2 (walk.cons step3 (walk.cons step4 walk.nil))),
+
+  have step1 : plane.adj (0,0) (1,0) := by rw [plane, cartesian_product, Z]; norm_num,
+  have step2 : plane.adj (1,0) (1,1) := by rw [plane, cartesian_product, Z]; norm_num,
+  exact walk.cons step1 (walk.cons step2 walk.nil),
+
+  have step1 : plane.adj (0,2) (-1,2) := by rw [plane, cartesian_product, Z]; norm_num,
+  have step2 : plane.adj (-1,2) (-1,1) := by rw [plane, cartesian_product, Z]; norm_num,
+  have step3 : plane.adj (-1,1) (-1,0) := by rw [plane, cartesian_product, Z]; norm_num,
+  have step4 : plane.adj (-1,0) (0,0) := by rw [plane, cartesian_product, Z]; norm_num,
+  exact walk.cons step1 (walk.cons step2 (walk.cons step3 (walk.cons step4 walk.nil))),
+  
+  have step1 : plane.adj (0,2) (1,2) := by rw [plane, cartesian_product, Z]; norm_num,
+  have step2 : plane.adj (1,2) (1,1) := by rw [plane, cartesian_product, Z]; norm_num,
+  exact walk.cons step1 (walk.cons step2 walk.nil),
+  
+  have step1 : plane.adj (1,1) (1,0) := by rw [plane, cartesian_product, Z]; norm_num,
+  have step2 : plane.adj (1,0) (0,0) := by rw [plane, cartesian_product, Z]; norm_num,
+  exact walk.cons step1 (walk.cons step2 walk.nil),
+  
+  have step1 : plane.adj (1,1) (1,2) := by rw [plane, cartesian_product, Z]; norm_num,
+  have step2 : plane.adj (1,2) (0,2) := by rw [plane, cartesian_product, Z]; norm_num,
+  exact walk.cons step1 (walk.cons step2 walk.nil),
+end
+
+lemma paths_support_nodup : ∀ e : K4.dart, (K4_dart_to_path e).support.nodup :=
+begin
+  rintro ⟨⟨e1, e2⟩, adj⟩,
+  fin_cases e1; fin_cases e2,
+  all_goals { dec_trivial, },
+end
+
+lemma no_overlap (e e' : K4.dart)
+                 (z : ℤ × ℤ)
+                 (hz1 : z ∈ (K4_dart_to_path e).support)
+                 (hz2 : z ∈ (K4_dart_to_path e').support) : (e.edge = e'.edge ∨ ∃ (x : ↥(finset.range 4)), z = K4_to_plane x) :=
+begin
+  rcases e with ⟨⟨ a1, a2 ⟩, adj_a⟩,
+  rcases e' with ⟨⟨ b1, b2 ⟩, adj_b⟩,
+
+  fin_cases a1; fin_cases a2,
+
+  all_goals {
+    fin_cases b1; fin_cases b2,
+
+    any_goals {
+      apply or.inl,
+      trivial <|> exact sym2.eq_swap,
+    },
+
+    all_goals { apply or.inr, },
+
+    all_goals {
+      iterate {erw [list.mem_cons_iff] at hz1},
+      iterate {erw [list.mem_cons_iff] at hz2},
+      rw list.mem_nil_iff at hz1 hz2,
+      cases_matching* [_ ∨ _],
+      any_goals {
+        exfalso,
+        assumption,
+      },
+      try { any_goals {
+          exfalso,
+          let p := prod.mk.inj (eq.trans (eq.symm hz1) hz2),
+          linarith [p.left, p.right],
+      }, },
+      try { any_goals {
+        use ⟨ 0, dec_trivial ⟩,
+        assumption,
+      }, },
+      try { any_goals {
+        use ⟨ 1, dec_trivial ⟩,
+        assumption,
+      }, },
+      try { any_goals {
+        use ⟨ 2, dec_trivial ⟩,
+        assumption,
+      }, },
+      try { any_goals {
+        use ⟨ 3, dec_trivial ⟩,
+        assumption,
+      }, },
+      done,
+    },
+  },
+end
+
+example : K4.is_planar :=
+begin
+  split,
+  {
+    refine nonempty.intro (path_embedding.mk _ _ _ _ _ _),
+    exact ⟨ K4_to_plane, (by dec_trivial!) ⟩,
+    exact K4_dart_to_path,
+    focus {
+      exact paths_support_nodup,
+    },
+    focus {
+      rintro ⟨⟨e1, e2⟩, adj⟩,
+      fin_cases e1; fin_cases e2,
+      all_goals { dec_trivial, },
+    },
+    focus {
+      rintro ⟨⟨e1, e2⟩, adj⟩,
+      fin_cases e1; fin_cases e2,
+      all_goals { dec_trivial, },
+    },
+    exact no_overlap,
+  },
+  split,
+  {
+    intros x y,
+    by_cases h : (x=y),
+    rwa h,
+    exact nonempty.intro (walk.cons (h) walk.nil),
+  },
+  {
+    apply (finset.nonempty_coe_sort (finset.range 4)).mpr,
+    apply (@finset.nonempty_range_iff 4).mpr,
+    norm_num,
+  }
+end
+
+end simple_graph
